dev/lf/delayed-types/Safety.v
@@ -198,6 +198,22 @@ Proof.
         eauto. eapply wf_stack_to_ok_S. subst. eauto.
       * assumption.
       * assumption.
+    + (* ifnull *)
+      specialize (IHty_trm Hwf). destruct IHty_trm as [IH | IH]; auto. inversion IH.
+      destruct IH as [sta' [sto' [t' [G' [G'' [S' [S'' [IH1 [IH2 [IH3 [IH4 [IH5 IH6]]]]]]]]]]]].
+      exists sta' sto' (trm_let t' u) G' G''. exists S' S''.
+      repeat split. 
+      * apply red_let_tgt. assumption.
+      * assumption. 
+      * assumption. 
+      * apply ty_let with (L:=L \u dom G') (T:=T); eauto. intros. 
+        rewrite IH3. apply weaken_ty_trm_sigma.
+        rewrite IH2. eapply (proj41 weaken_rules_ctx). apply H0. auto. 
+        reflexivity.
+        rewrite <- IH2. apply ok_push. eapply wf_stack_to_ok_G. eassumption. 
+        eauto. eapply wf_stack_to_ok_S. subst. eauto.
+      * assumption.
+      * assumption.
   - specialize (IHty_trm Hwf). destruct IHty_trm as [IH | IH]; auto.
     right. destruct IH as [sta' [sto' [t' [G' [G'' [S' [S'' [IH1 [IH2 [IH3 [IH4 [IH5 IH6]]]]]]]]]]]].
     exists sta' sto' t' G' G''. exists S' S''.
@@ -227,31 +243,31 @@ Proof.
     split. rewrite concat_empty_r. reflexivity.
     split. rewrite concat_empty_r. reflexivity.
     split. assumption. split. assumption. assumption.
-  - (* asg_ref *)
-    right.
-    pose proof (canonical_forms_3 Hg Hwf Hwt H) as [l [y' [BiLoc [Hty [BiSto Htyy']]]]].
-    exists sta (sto[l := y]) (trm_var (avar_f x)) G (@empty typ). exists S (@empty typ).
-    split.
-    + apply red_asgn with (l:=l).
-      * assumption.
-      * lets Hbd: (LibMap.binds_def sto l y'). unfold bindsM in BiSto. rewrite Hbd in BiSto.
-        destruct BiSto as [His Hsto]. assumption.
-    + repeat split.
-      * rewrite concat_empty_r. reflexivity.
-      * rewrite concat_empty_r. reflexivity.
-      * assumption.
-      * assumption.
-      * pose proof (general_to_tight Hg) as [A _].
-        pose proof (A ty_general sub_general G S (trm_var (avar_f x)) (typ_ref T) H eq_refl eq_refl eq_refl).
-        pose proof (A ty_general sub_general G S (trm_val (val_loc l)) (typ_ref T) Hty eq_refl eq_refl eq_refl).
-        destruct (precise_ref_subtyping Hg BiLoc H1 H2 Hwf Hwt) as [U [HU [Hs1 Hs2]]].
-        apply wt_store_update with (T:=U); try assumption.
-        apply (ref_binds_typ HU). apply ty_sub with (T:=T); assumption.
+  (* - (* asg_ref *) *)
+  (*   right. *)
+  (*   pose proof (canonical_forms_3 Hg Hwf Hwt H) as [l [y' [BiLoc [Hty [BiSto Htyy']]]]]. *)
+  (*   exists sta (sto[l := y]) (trm_var (avar_f x)) G (@empty typ). exists S (@empty typ). *)
+  (*   split. *)
+  (*   + apply red_asgn with (l:=l). *)
+  (*     * assumption. *)
+  (*     * lets Hbd: (LibMap.binds_def sto l y'). unfold bindsM in BiSto. rewrite Hbd in BiSto. *)
+  (*       destruct BiSto as [His Hsto]. assumption. *)
+  (*   + repeat split. *)
+  (*     * rewrite concat_empty_r. reflexivity. *)
+  (*     * rewrite concat_empty_r. reflexivity. *)
+  (*     * assumption. *)
+  (*     * assumption. *)
+  (*     * pose proof (general_to_tight Hg) as [A _]. *)
+  (*       pose proof (A ty_general sub_general G S (trm_var (avar_f x)) (typ_ref T) H eq_refl eq_refl eq_refl). *)
+  (*       pose proof (A ty_general sub_general G S (trm_val (val_loc l)) (typ_ref T) Hty eq_refl eq_refl eq_refl). *)
+  (*       destruct (precise_ref_subtyping Hg BiLoc H1 H2 Hwf Hwt) as [U [HU [Hs1 Hs2]]]. *)
+  (*       apply wt_store_update with (T:=U); try assumption. *)
+  (*       apply (ref_binds_typ HU). apply ty_sub with (T:=T); assumption. *)
   - (* asgn_nref *)
     right.
     exists sta sto (trm_var (avar_f x)) G (@empty typ). exists S (@empty typ).
     (* pose proof (canonical_forms_3 Hg Hwf Hwt H) as [l [y' [BiLoc [Hty [BiSto Htyy']]]]]. *)
-    exists sta (sto[l := y]) (trm_var (avar_f x)) G (@empty typ). exists S (@empty typ).
+    (* exists sta (sto[l := y]) (trm_var (avar_f x)) G (@empty typ). exists S (@empty typ). *)
     split.
     + apply red_asgn with (l:=l).
       * assumption.
